- $(\neg (\neg E \land A) \lor B) \land \neg ((C \land E) \land (D \lor E))$
- $\neg ((B \land C) \lor (\neg C \implies D)) \implies \neg B$
- $\neg C \lor ((A \iff E) \lor D)$
- $((B \lor E) \lor D) \lor ((D \iff C) \land \neg (\neg B \lor D))$
- $((D \iff B) \lor (\neg E \lor D)) \implies D$
- $(E \implies (A \iff D)) \land B$
- $(D \land \neg (B \iff \neg C)) \implies E$
- $\neg ((C \iff D) \implies (\neg A \iff D)) \lor ((\neg D \implies C) \land (\neg B \lor A))$
- $\neg B \land A$
- $(B \iff D) \land A$
- $(\neg (B \implies D) \land \neg (\neg D \lor B)) \implies A$
- $(\neg B \lor (B \land \neg E)) \implies \neg ((\neg E \implies C) \lor (\neg E \iff D))$
- $B \lor A$
- $\neg ((C \land \neg E) \iff (B \lor A)) \iff (\neg (\neg D \iff B) \lor (A \lor D))$
- $E \lor B$
- $((D \iff E) \lor \neg (\neg A \iff E)) \iff ((C \lor E) \lor \neg (\neg D \iff A))$
- $(A \lor \neg B) \implies (B \lor (D \implies E))$
- $(A \lor (B \lor D)) \land ((D \iff C) \lor D)$
- $(\neg A \lor (D \iff \neg E)) \lor (\neg D \iff \neg C)$
- $D \land (B \lor \neg (B \land D))$
- $E \lor (D \implies \neg (E \lor B))$
- $\neg (B \iff (E \implies A)) \implies \neg C$
- $\neg (\neg (E \implies \neg A) \iff (\neg C \iff \neg B)) \iff \neg ((\neg B \lor A) \lor (\neg C \lor \neg D))$
- $E \land (\neg (B \lor \neg D) \lor (\neg A \iff D))$
- $(C \land (C \implies A)) \lor ((\neg B \lor \neg C) \lor \neg A)$
- $(\neg A \implies \neg (E \implies D)) \land E$
- $B \land ((D \iff A) \land \neg (D \lor A))$
- $\neg (\neg (\neg B \land D) \lor (D \implies A)) \land (\neg (A \land E) \land (B \implies C))$
- $\neg C \lor A$
- $C \lor ((D \implies B) \land (\neg B \implies \neg D))$
